implamented PointwisePredicate function and used it.

SliceRefinements.dfy
@@ -361,6 +361,11 @@ ensures CoSliceRefinement(S1, S2, V) <==> (forall P: Predicate,s: State :: (vars
 //============================================================
 //					*** Predicate Operators ***
 //============================================================
+function PointwisePredicate(s: State, v: Variable) : Predicate
+{
+	(((s1: State) reads*  => v in s1 && v in s && s[v] == s1[v] ,{v}))
+}
+
 function AND(P1: Predicate,P2: Predicate): Predicate
 {
 	((s: State) reads * requires P1.0.requires(s) && P2.0.requires(s) => P1.0(s) && P2.0(s),P1.1 + P2.1)
@@ -426,7 +431,7 @@ ensures EquivalentPredicates(P,(((s1: State) reads * requires P.0.requires(s1) =
 lemma Equation_5_2(S: Statement, Sco: Statement, V: set<Variable>)
 requires Valid(S)
 requires Valid(Sco)
-ensures (forall s: State, v: Variable :: v in V && v in s ==> var P:= (((s1: State) reads *  => v in s1 && s[v] == s1[v]),{v}); (wp(S,P).0(s) ==> wp(Sco,P).0(s)))
+ensures (forall s: State, v: Variable :: v in V && v in s ==> (wp(S,PointwisePredicate(s,v)).0(s) ==> wp(Sco,PointwisePredicate(s,v)).0(s)))
 
 //============================================================
 //					*** RE1-RE5 ***
@@ -664,7 +669,7 @@ lemma RE5(S: Statement)
 }
 */
  
-//TODO: pointwisePredicate -< dummmy 6 (forall s: State :: ((wp(S,ConstantPredicate(true)).0(s) ==> wp(SV,ConstantPredicate(true)).0(s)))) && (forall s: State ,x: Variable :: x in (V) && x in s ==> var P := ((s1: state) /* requires (x in s1)*/ => s[x] == s1[x] ,{x}); (wp(S,P).0(s) ==> wp(SV,P).0(s)))
+
 
 //============================================================
 //					*** THEOREMS ***
@@ -725,13 +730,13 @@ reads *
 requires Valid(S)
 requires Valid(SV)
 {
-	(forall s: State :: ((wp(S,ConstantPredicate(true)).0(s) ==> wp(SV,ConstantPredicate(true)).0(s)))) && (forall s: State, v: Variable :: v in V && v in s ==> var P:= (((s1: State) reads *  => v in s1 && v in s && s[v] == s1[v]),{v}); (wp(S,P).0(s) ==> wp(SV,P).0(s)))
+	(forall s: State :: ((wp(S,ConstantPredicate(true)).0(s) ==> wp(SV,ConstantPredicate(true)).0(s)))) && (forall s: State, v: Variable :: v in V && v in s ==> (wp(S,PointwisePredicate(s,v)).0(s) ==> wp(SV,PointwisePredicate(s,v)).0(s)))
 }
 
 lemma dummy7Lemma(S: Statement, SV: Statement, V: set<Variable>)
 requires Valid(S)
 requires Valid(SV)
-ensures dummy7(S,SV,V) <==> (forall s: State :: ((wp(S,ConstantPredicate(true)).0(s) ==> wp(SV,ConstantPredicate(true)).0(s)))) && (forall s: State, v: Variable :: v in V && v in s ==> var P:= (((s1: State) reads *  => v in s1 && v in s && s[v] == s1[v]),{v}); (wp(S,P).0(s) ==> wp(SV,P).0(s)))
+ensures dummy7(S,SV,V) <==> (forall s: State :: ((wp(S,ConstantPredicate(true)).0(s) ==> wp(SV,ConstantPredicate(true)).0(s)))) && (forall s: State, v: Variable :: v in V && v in s ==> (wp(S,PointwisePredicate(s,v)).0(s) ==> wp(SV,PointwisePredicate(s,v)).0(s)))
 
 
 lemma {:verify true} Theorem_5_1 (S: Statement, SV: Statement, V: set<Variable>)
@@ -820,14 +825,13 @@ reads *
 requires Valid(S)
 requires Valid(SV)
 {
-	(((forall s: State :: ((wp(S,ConstantPredicate(true)).0(s) ==> wp(SV,ConstantPredicate(true)).0(s)))) && (forall s: State, v: Variable :: v in (def(S)+def(SV)-V) && v in s ==> var P:= (((s1: State) reads *  => v in s1 && v in s && s[v] == s1[v]),{v}); (wp(S,P).0(s) ==> wp(SV,P).0(s)))))
+	(((forall s: State :: ((wp(S,ConstantPredicate(true)).0(s) ==> wp(SV,ConstantPredicate(true)).0(s)))) && (forall s: State, v: Variable :: v in (def(S)+def(SV)-V) && v in s ==> (wp(S,PointwisePredicate(s,v)).0(s) ==> wp(SV,PointwisePredicate(s,v)).0(s)))))
 }
 
 lemma dummy3Lemma(S: Statement, SV: Statement, V: set<Variable>)
 requires Valid(S)
 requires Valid(SV)
-ensures dummy3(S,SV,V) <==> (((forall s: State :: ((wp(S,ConstantPredicate(true)).0(s) ==> wp(SV,ConstantPredicate(true)).0(s)))) && (forall s: State, v: Variable :: v in (def(S)+def(SV)-V) && v in s ==> var P:= (((s1: State) reads *  => v in s1 && v in s && s[v] == s1[v]),{v}); (wp(S,P).0(s) ==> wp(SV,P).0(s)))))
-						//    (forall s: State :: ((wp(S,ConstantPredicate(true)).0(s) ==> wp(SV,ConstantPredicate(true)).0(s)))) && (forall s: State ,v: Variable :: v in (def(S)+def(SV)-V) && v in s ==> var P := ((s1: State) reads * => v in s1 && v in s && s[v] == s1[v],{v}); (wp(S,P).0(s) ==> wp(SV,P).0(s)));																			
+ensures dummy3(S,SV,V) <==> (((forall s: State :: ((wp(S,ConstantPredicate(true)).0(s) ==> wp(SV,ConstantPredicate(true)).0(s)))) && (forall s: State, v: Variable :: v in (def(S)+def(SV)-V) && v in s ==> (wp(S,PointwisePredicate(s,v)).0(s) ==> wp(SV,PointwisePredicate(s,v)).0(s)))))
 
 lemma {:verify true} Corollary_5_2 (S: Statement, SV: Statement, V: set<Variable>)
 requires Valid(S)
@@ -839,7 +843,7 @@ ensures (CoSliceRefinement(S,SV,V)) <==> dummy3(S,SV,V)
 	== {Corollary_5_3(S,SV,V,(def(S) + def(SV)) - V);}
 	SliceRefinement(S,SV,(def(S) + def(SV)) - V);
 	== {Theorem_5_1(S,SV,(def(S) + def(SV)) - V);dummy7Lemma(S,SV,(def(S) + def(SV)) - V);}
-	((forall s:State :: ((wp(S,ConstantPredicate(true)).0(s) ==> wp(SV,ConstantPredicate(true)).0(s)))) && (forall s: State, v: Variable :: v in (def(S)+def(SV)-V) && v in s ==> var P:= (((s1: State) reads *  => v in s1 && v in s && s[v] == s1[v]),{v}); (wp(S,P).0(s) ==> wp(SV,P).0(s))));
+	((forall s:State :: ((wp(S,ConstantPredicate(true)).0(s) ==> wp(SV,ConstantPredicate(true)).0(s)))) && (forall s: State, v: Variable :: v in (def(S)+def(SV)-V) && v in s ==> (wp(S,PointwisePredicate(s,v)).0(s) ==> wp(SV,PointwisePredicate(s,v)).0(s))));
 	== {dummy3Lemma(S,SV,V);}
 	dummy3(S,SV,V);
 	}
@@ -901,13 +905,13 @@ reads *
 requires Valid(S)
 requires Valid(SV)
 {
-	(forall s: State :: ((wp(S,ConstantPredicate(true)).0(s) ==> wp(SV,ConstantPredicate(true)).0(s)))) && (forall s: State ,v: Variable :: v in (V+def(S)+def(SV)) && v in s  ==> var P := (((s1: State)  reads * => v in s1 && v in s && s[v] == s1[v]),{v}); (wp(S,P).0(s) ==> wp(SV,P).0(s)))
+	(forall s: State :: ((wp(S,ConstantPredicate(true)).0(s) ==> wp(SV,ConstantPredicate(true)).0(s)))) && (forall s: State ,v: Variable :: v in (V+def(S)+def(SV)) && v in s  ==> (wp(S,PointwisePredicate(s,v)).0(s) ==> wp(SV,PointwisePredicate(s,v)).0(s)))
 }
 
 lemma dummy4Lemma(S: Statement, SV: Statement, V: set<Variable>)
 requires Valid(S)
 requires Valid(SV)
-ensures dummy4(S,SV,V) <==> (forall s: State :: ((wp(S,ConstantPredicate(true)).0(s) ==> wp(SV,ConstantPredicate(true)).0(s)))) && (forall s: State ,v: Variable :: v in (V+def(S)+def(SV)) && v in s  ==> var P := ((s1: State)  reads * => v in s1 && v in s && s[v] == s1[v],{v}); (wp(S,P).0(s) ==> wp(SV,P).0(s)))
+ensures dummy4(S,SV,V) <==> (forall s: State :: ((wp(S,ConstantPredicate(true)).0(s) ==> wp(SV,ConstantPredicate(true)).0(s)))) && (forall s: State ,v: Variable :: v in (V+def(S)+def(SV)) && v in s  ==> (wp(S,PointwisePredicate(s,v)).0(s) ==> wp(SV,PointwisePredicate(s,v)).0(s)))
 
 // TODO: complete 3 error : 2 assemption to use 5.5 -> why is it valid to all ranges?
 lemma {:verify false} dummy4AllRange(S: Statement, SV: Statement, V: set<Variable>)
@@ -919,13 +923,13 @@ ensures dummy3(S,SV,{}) <==>  dummy4(S,SV,V)
 	calc {
 	dummy3(S,SV,{});
 	== {dummy3Lemma(S,SV,{});}
-	(((forall s: State :: ((wp(S,ConstantPredicate(true)).0(s) ==> wp(SV,ConstantPredicate(true)).0(s)))) && (forall s: State, v: Variable :: v in (def(S)+def(SV)-{}) && v in s ==> var P := ((s1: State)  reads * => v in s1 && v in s && s[v] == s1[v],{v}); (wp(S,P).0(s) ==> wp(SV,P).0(s)))));
+	(((forall s: State :: ((wp(S,ConstantPredicate(true)).0(s) ==> wp(SV,ConstantPredicate(true)).0(s)))) && (forall s: State, v: Variable :: v in (def(S)+def(SV)-{}) && v in s ==> (wp(S,PointwisePredicate(s,v)).0(s) ==> wp(SV,PointwisePredicate(s,v)).0(s)))));
 	== {}
-	((forall s: State :: ((wp(S,ConstantPredicate(true)).0(s) ==> wp(SV,ConstantPredicate(true)).0(s)))) && (forall s: State ,v: Variable :: v in (def(S)+def(SV)) && v in s ==> var P := ((s1: State)  reads * => v in s1 && v in s && s[v] == s1[v],{v}); (wp(S,P).0(s) ==> wp(SV,P).0(s))));
+	((forall s: State :: ((wp(S,ConstantPredicate(true)).0(s) ==> wp(SV,ConstantPredicate(true)).0(s)))) && (forall s: State ,v: Variable :: v in (def(S)+def(SV)) && v in s ==> (wp(S,PointwisePredicate(s,v)).0(s) ==> wp(SV,PointwisePredicate(s,v)).0(s))));
 	== {var P:=  (((s1: State) reads *  =>  v in (def(S)+def(SV)-{}) && v in s && v in s1 && s[v] == s1[v]),{v}); assert vars(P) !! (def(S) + def(SV)); assert (forall s: State :: ((wp(S,ConstantPredicate(true)).0(s) ==> wp(SV,ConstantPredicate(true)).0(s)))); Corollary_5_5(S, SV,P);}
-	((forall s: State :: ((wp(S,ConstantPredicate(true)).0(s) ==> wp(SV,ConstantPredicate(true)).0(s)))) && (forall s: State ,v: Variable :: v in (def(S)+def(SV)) && v in s ==> var P := ((s1: State)  reads * => v in s1 && v in s && s[v] == s1[v],{v}); (wp(S,P).0(s) ==> wp(SV,P).0(s)))) && (forall s: State ,v: Variable :: v in (V - (def(S)+def(SV))) && v in s ==> var P := ((s1: State)  reads * => v in s1 && v in s && s[v] == s1[v],{v}); (wp(S,P).0(s) ==> wp(SV,P).0(s)));
+	((forall s: State :: ((wp(S,ConstantPredicate(true)).0(s) ==> wp(SV,ConstantPredicate(true)).0(s)))) && (forall s: State ,v: Variable :: v in (def(S)+def(SV)) && v in s ==> (wp(S,PointwisePredicate(s,v)).0(s) ==> wp(SV,PointwisePredicate(s,v)).0(s)))) && (forall s: State ,v: Variable :: v in (V - (def(S)+def(SV))) && v in s ==> (wp(S,PointwisePredicate(s,v)).0(s) ==> wp(SV,PointwisePredicate(s,v)).0(s)));
 	== {}
-	((forall s: State :: ((wp(S,ConstantPredicate(true)).0(s) ==> wp(SV,ConstantPredicate(true)).0(s)))) && (forall s: State ,v: Variable :: v in (V + def(S)+def(SV)) && v in s ==> var P := ((s1: State)  reads * => v in s1 && v in s && s[v] == s1[v],{v}); (wp(S,P).0(s) ==> wp(SV,P).0(s))));
+	((forall s: State :: ((wp(S,ConstantPredicate(true)).0(s) ==> wp(SV,ConstantPredicate(true)).0(s)))) && (forall s: State ,v: Variable :: v in (V + def(S)+def(SV)) && v in s ==> (wp(S,PointwisePredicate(s,v)).0(s) ==> wp(SV,PointwisePredicate(s,v)).0(s))));
 	== {dummy4Lemma(S,SV,V);}
 	dummy4(S,SV,V);
 	}
@@ -941,11 +945,11 @@ ensures dummy4(S,SV,V) <==> dummy5(S,SV,V)
 	calc {
 		dummy4(S,SV,V);
 		== {dummy4Lemma(S,SV,V);}
-		(forall s: State :: ((wp(S,ConstantPredicate(true)).0(s) ==> wp(SV,ConstantPredicate(true)).0(s)))) && (forall s: State ,v: Variable :: v in (V+def(S)+def(SV)) && v in s  ==> var P := ((s1: State)  reads * => v in s1 && v in s && s[v] == s1[v],{v}); (wp(S,P).0(s) ==> wp(SV,P).0(s)));
+		(forall s: State :: ((wp(S,ConstantPredicate(true)).0(s) ==> wp(SV,ConstantPredicate(true)).0(s)))) && (forall s: State ,v: Variable :: v in (V+def(S)+def(SV)) && v in s  ==> (wp(S,PointwisePredicate(s,v)).0(s) ==> wp(SV,PointwisePredicate(s,v)).0(s)));
 		== {}
-		(forall s: State :: ((wp(S,ConstantPredicate(true)).0(s) ==> wp(SV,ConstantPredicate(true)).0(s)))) && (forall s: State ,v: Variable :: (v in (V) || v in (def(S)+def(SV))) && v in s  ==> var P := ((s1: State)  reads * => v in s1 && v in s && s[v] == s1[v],{v}); (wp(S,P).0(s) ==> wp(SV,P).0(s)));
+		(forall s: State :: ((wp(S,ConstantPredicate(true)).0(s) ==> wp(SV,ConstantPredicate(true)).0(s)))) && (forall s: State ,v: Variable :: (v in (V) || v in (def(S)+def(SV))) && v in s  ==> (wp(S,PointwisePredicate(s,v)).0(s) ==> wp(SV,PointwisePredicate(s,v)).0(s)));
 		== {}
-		(forall s: State :: ((wp(S,ConstantPredicate(true)).0(s) ==> wp(SV,ConstantPredicate(true)).0(s)))) && (forall s: State ,v: Variable :: v in (V) && v in s ==> var P := ((s1: State)  reads * => v in s1 && v in s && s[v] == s1[v],{v}); (wp(S,P).0(s) ==> wp(SV,P).0(s))) && (forall s: State ,v: Variable :: v in ((def(S)+def(SV))-V)  ==> var P := ((s1: State)  reads * => v in s1 && v in s && s[v] == s1[v],{v}); (wp(S,P).0(s) ==> wp(SV,P).0(s)));
+		(forall s: State :: ((wp(S,ConstantPredicate(true)).0(s) ==> wp(SV,ConstantPredicate(true)).0(s)))) && (forall s: State ,v: Variable :: v in (V) && v in s ==> (wp(S,PointwisePredicate(s,v)).0(s) ==> wp(SV,PointwisePredicate(s,v)).0(s))) && (forall s: State ,v: Variable :: v in ((def(S)+def(SV))-V)  ==> (wp(S,PointwisePredicate(s,v)).0(s) ==> wp(SV,PointwisePredicate(s,v)).0(s)));
 		== {dummy5Lemma(S,SV,V);}
 		dummy5(S,SV,V);
 	}
@@ -957,13 +961,13 @@ reads *
 requires Valid(S)
 requires Valid(SV)
 {
-	(forall s: State :: ((wp(S,ConstantPredicate(true)).0(s) ==> wp(SV,ConstantPredicate(true)).0(s)))) && (forall s: State ,v: Variable :: v in (V) && v in s ==> var P := ((s1: State)  reads * => v in s1 && v in s && s[v] == s1[v],{v}); (wp(S,P).0(s) ==> wp(SV,P).0(s))) && (forall s: State ,v: Variable :: v in ((def(S)+def(SV))-V)  ==> var P := ((s1: State)  reads * => v in s1 && v in s && s[v] == s1[v],{v}); (wp(S,P).0(s) ==> wp(SV,P).0(s)))
+	(forall s: State :: ((wp(S,ConstantPredicate(true)).0(s) ==> wp(SV,ConstantPredicate(true)).0(s)))) && (forall s: State ,v: Variable :: v in (V) && v in s ==> (wp(S,PointwisePredicate(s,v)).0(s) ==> wp(SV,PointwisePredicate(s,v)).0(s))) && (forall s: State ,v: Variable :: v in ((def(S)+def(SV))-V)  ==> (wp(S,PointwisePredicate(s,v)).0(s) ==> wp(SV,PointwisePredicate(s,v)).0(s)))
 }
 
 lemma dummy5Lemma(S: Statement, SV: Statement, V: set<Variable>)
 requires Valid(S)
 requires Valid(SV)
-ensures dummy5(S,SV,V) <==> (forall s: State :: ((wp(S,ConstantPredicate(true)).0(s) ==> wp(SV,ConstantPredicate(true)).0(s)))) && (forall s: State ,v: Variable :: v in (V) && v in s ==> var P := ((s1: State)  reads * => v in s1 && v in s && s[v] == s1[v],{v}); (wp(S,P).0(s) ==> wp(SV,P).0(s))) && (forall s: State ,v: Variable :: v in ((def(S)+def(SV))-V)  ==> var P := ((s1: State)  reads * => v in s1 && v in s && s[v] == s1[v],{v}); (wp(S,P).0(s) ==> wp(SV,P).0(s)))
+ensures dummy5(S,SV,V) <==> (forall s: State :: ((wp(S,ConstantPredicate(true)).0(s) ==> wp(SV,ConstantPredicate(true)).0(s)))) && (forall s: State ,v: Variable :: v in (V) && v in s ==> (wp(S,PointwisePredicate(s,v)).0(s) ==> wp(SV,PointwisePredicate(s,v)).0(s))) && (forall s: State ,v: Variable :: v in ((def(S)+def(SV))-V)  ==> (wp(S,PointwisePredicate(s,v)).0(s) ==> wp(SV,PointwisePredicate(s,v)).0(s)))
 
 lemma dummy5dummy6Lemma(S: Statement, SV: Statement, V: set<Variable>,CoV: set<Variable>)
 requires Valid(S)
@@ -978,7 +982,7 @@ requires Valid(S)
 requires Valid(SV)
 requires CoV == (def(S) + def(SV)) - V
 {
-	(forall s: State :: ((wp(S,ConstantPredicate(true)).0(s) ==> wp(SV,ConstantPredicate(true)).0(s)))) && (forall s: State ,v: Variable :: v in (V) && v in s ==> var P := ((s1: State)  reads * => v in s1 && v in s && s[v] == s1[v],{v}); (wp(S,P).0(s) ==> wp(SV,P).0(s)))
+	(forall s: State :: ((wp(S,ConstantPredicate(true)).0(s) ==> wp(SV,ConstantPredicate(true)).0(s)))) && (forall s: State ,v: Variable :: v in (V) && v in s ==> (wp(S,PointwisePredicate(s,v)).0(s) ==> wp(SV,PointwisePredicate(s,v)).0(s)))
 }
 
 predicate CoDummy6(S: Statement, SV: Statement, V: set<Variable>,CoV: set<Variable>)
@@ -987,7 +991,7 @@ requires Valid(S)
 requires Valid(SV)
 requires CoV == (def(S) + def(SV)) - V
 {
-	(forall s: State :: ((wp(S,ConstantPredicate(true)).0(s) ==> wp(SV,ConstantPredicate(true)).0(s)))) && (forall s: State ,v: Variable :: v in (CoV) && v in s ==> var P := ((s1: State)  reads * => v in s1 && v in s && s[v] == s1[v],{v}); (wp(S,P).0(s) ==> wp(SV,P).0(s)))
+	(forall s: State :: ((wp(S,ConstantPredicate(true)).0(s) ==> wp(SV,ConstantPredicate(true)).0(s)))) && (forall s: State ,v: Variable :: v in (CoV) && v in s ==> (wp(S,PointwisePredicate(s,v)).0(s) ==> wp(SV,PointwisePredicate(s,v)).0(s)))
 }
 
 
@@ -995,13 +999,13 @@ lemma dummy6Lemma(S: Statement, SV: Statement, V: set<Variable>,CoV: set<Variabl
 requires Valid(S)
 requires Valid(SV)
 requires CoV == (def(S) + def(SV)) - V
-ensures dummy6(S,SV,V,CoV) <==> (forall s: State :: ((wp(S,ConstantPredicate(true)).0(s) ==> wp(SV,ConstantPredicate(true)).0(s)))) && (forall s: State ,v: Variable :: v in (V) && v in s ==> var P := ((s1: State) reads * => v in s1 && v in s && s[v] == s1[v],{v}); (wp(S,P).0(s) ==> wp(SV,P).0(s)))
+ensures dummy6(S,SV,V,CoV) <==> (forall s: State :: ((wp(S,ConstantPredicate(true)).0(s) ==> wp(SV,ConstantPredicate(true)).0(s)))) && (forall s: State ,v: Variable :: v in (V) && v in s ==> (wp(S,PointwisePredicate(s,v)).0(s) ==> wp(SV,PointwisePredicate(s,v)).0(s)))
 
 lemma CoDummy6Lemma(S: Statement, SV: Statement, V: set<Variable>,CoV: set<Variable>)
 requires Valid(S)
 requires Valid(SV)
 requires CoV == (def(S) + def(SV)) - V
-ensures CoDummy6(S,SV,V,CoV) <==> (forall s: State :: ((wp(S,ConstantPredicate(true)).0(s) ==> wp(SV,ConstantPredicate(true)).0(s)))) && (forall s: State ,v: Variable :: v in (CoV) && v in s ==> var P := ((s1: State) reads * => v in s1 && v in s && s[v] == s1[v],{v}); (wp(S,P).0(s) ==> wp(SV,P).0(s)))
+ensures CoDummy6(S,SV,V,CoV) <==> (forall s: State :: ((wp(S,ConstantPredicate(true)).0(s) ==> wp(SV,ConstantPredicate(true)).0(s)))) && (forall s: State ,v: Variable :: v in (CoV) && v in s ==> (wp(S,PointwisePredicate(s,v)).0(s) ==> wp(SV,PointwisePredicate(s,v)).0(s)))
 
 // TODO: Complete 1 err
 lemma {:verify true} CoDummy6CoSliceRefinementLemma(S: Statement, SV: Statement, V: set<Variable>,CoV: set<Variable>)
@@ -1013,9 +1017,9 @@ ensures CoSliceRefinement(S,SV,V) <==> CoDummy6(S,SV,V,CoV)
 	calc {
 		CoDummy6(S,SV,V,CoV);
 		== {CoDummy6Lemma(S,SV,V,CoV);}
-		(forall s: State :: ((wp(S,ConstantPredicate(true)).0(s) ==> wp(SV,ConstantPredicate(true)).0(s)))) && (forall s: State ,v: Variable :: v in (CoV) && v in s ==> var P := ((s1: State) reads * => v in s1 && v in s && s[v] == s1[v],{v}); (wp(S,P).0(s) ==> wp(SV,P).0(s)));
+		(forall s: State :: ((wp(S,ConstantPredicate(true)).0(s) ==> wp(SV,ConstantPredicate(true)).0(s)))) && (forall s: State ,v: Variable :: v in (CoV) && v in s ==> (wp(S,PointwisePredicate(s,v)).0(s) ==> wp(SV,PointwisePredicate(s,v)).0(s)));
 		== {assert CoV == (def(S)+def(SV)-V);}
-		(forall s: State :: ((wp(S,ConstantPredicate(true)).0(s) ==> wp(SV,ConstantPredicate(true)).0(s)))) && (forall s: State ,v: Variable :: v in (def(S)+def(SV)-V) && v in s ==> var P := ((s1: State) reads * => v in s1 && v in s && s[v] == s1[v],{v}); (wp(S,P).0(s) ==> wp(SV,P).0(s)));
+		(forall s: State :: ((wp(S,ConstantPredicate(true)).0(s) ==> wp(SV,ConstantPredicate(true)).0(s)))) && (forall s: State ,v: Variable :: v in (def(S)+def(SV)-V) && v in s ==> (wp(S,PointwisePredicate(s,v)).0(s) ==> wp(SV,PointwisePredicate(s,v)).0(s)));
 		== {dummy3Lemma(S,SV,V);}
 		dummy3(S,SV,V);
 		== {Corollary_5_2(S,SV,V);}
@@ -1033,10 +1037,10 @@ ensures SliceRefinement(S,SV,V) <==> dummy6(S,SV,V,CoV)
 	calc {
 		dummy6(S,SV,V,CoV);
 		=={dummy6Lemma(S,SV,V,CoV);}
-		(forall s: State :: ((wp(S,ConstantPredicate(true)).0(s) ==> wp(SV,ConstantPredicate(true)).0(s)))) && (forall s: State ,v: Variable :: v in (V) && v in s ==> var P := ((s1: State) reads * => v in s1 && v in s && s[v] == s1[v],{v}); (wp(S,P).0(s) ==> wp(SV,P).0(s)));
+		(forall s: State :: ((wp(S,ConstantPredicate(true)).0(s) ==> wp(SV,ConstantPredicate(true)).0(s)))) && (forall s: State ,v: Variable :: v in (V) && v in s ==> (wp(S,PointwisePredicate(s,v)).0(s) ==> wp(SV,PointwisePredicate(s,v)).0(s)));
 		== {}
-		(forall s: State :: ((wp(S,ConstantPredicate(true)).0(s) ==> wp(SV,ConstantPredicate(true)).0(s)))) && (forall s: State ,v: Variable :: v in (V) && v in s ==> var P := ((s1: State) reads * => v in s1 && v in s && s[v] == s1[v],{v}); (wp(S,P).0(s) ==> wp(SV,P).0(s)));
-	//	(forall s: State :: ((wp(S,ConstantPredicate(true)).0(s) ==> wp(SV,ConstantPredicate(true)).0(s)))) && (forall s: State, v: Variable :: v in V && v in s ==> var P:= (((s1: State) reads *  => v in s1 && v in s && s[v] == s1[v]),{v}); (wp(S,P).0(s) ==> wp(SV,P).0(s)))	
+		(forall s: State :: ((wp(S,ConstantPredicate(true)).0(s) ==> wp(SV,ConstantPredicate(true)).0(s)))) && (forall s: State ,v: Variable :: v in (V) && v in s ==> (wp(S,PointwisePredicate(s,v)).0(s) ==> wp(SV,PointwisePredicate(s,v)).0(s)));
+	//	(forall s: State :: ((wp(S,ConstantPredicate(true)).0(s) ==> wp(SV,ConstantPredicate(true)).0(s)))) && (forall s: State, v: Variable :: v in V && v in s ==> (wp(S,PointwisePredicate(s,v)).0(s) ==> wp(SV,PointwisePredicate(s,v)).0(s)))	
 		== {dummy7Lemma(S,SV,V);}
 		dummy7(S,SV,V);
 		=={Theorem_5_1(S,SV,V);}
